src/theory/QueryNormalFormLemmas.v
@@ -475,7 +475,7 @@ Section Normalisation.
    *)
   (* Conformance is not really needed... *)
   Lemma normalize_root_query_is_in_normal_form φ :
-    queries_conform s s.(query_type) φ ->
+    selections_conform s s.(query_type) φ ->
     are_non_redundant (normalize s s.(query_type) φ) /\
     are_grounded s (normalize s s.(query_type) φ).
   Proof.
